array reversal, modulo admits on two library lemmas on bigstar

src/examples/GPU.ArrayReversal.fst
@@ -7,64 +7,127 @@ open GPU
 open Pulse.Lib.BoundedIntegers
 open FStar.SizeT
 module SZ = FStar.SizeT
-let named (n:string) (x:slprop) = x
-fn intro_named (n:string) (x:slprop)
-requires x
-ensures named n x
-{
-  fold (named n x)
-}
 
-open FStar.OrdSet
+let index_flip (#a:Type) (s:seq a) (i:nat { i < Seq.length s }) = Seq.index s (Seq.length s - i - 1 <: nat)
+let reverse_spec (#a:Type) (s:seq a) = Seq.init (Seq.length s) (fun i -> index_flip s i)
+
+open FStar.FiniteSet.Base
+open FStar.FiniteSet.Ambient
+module Set = FStar.FiniteSet.Base
 let idx (m n:nat) = i:nat { m <= i /\ i < n }
-let idx_set (m n:nat) = FStar.OrdSet.ordset (idx m n) (fun (x y:nat) -> x <= y)
+let idx_set (m n:nat) = s:set nat { forall x. x `Set.mem` s ==> m <= x /\ x < n }
+let partitions (m:nat) (n:nat) (k:nat) = i:nat{ i < k } -> idx_set m n
+let select #m #n #k (p:partitions m n k) (i:nat{ i < k }) : idx_set m n = p i
 
-let partitions (m:nat) (n:nat) = seq (idx_set m n)
-let union_partitions #m #n (p:partitions m n) = FStar.Seq.foldr OrdSet.union p OrdSet.empty  
-let range (m:nat) (n:nat { m <= n }) : s:idx_set m n { forall i. OrdSet.mem i s <==> m <= i /\ i < n } =
-  let rec aux (k:nat { m <= k /\ k <= n }) 
-  : Tot (s:idx_set m n { forall i. OrdSet.mem i s <==> k <= i /\ i < n}) (decreases (n - k))
-  = if k = n then OrdSet.empty
-    else OrdSet.union (OrdSet.singleton k) (aux (k + 1 <: nat))
-  in
-  aux m
+let rec union_partitions_aux #m #n #k (p:partitions m n k) (from:nat) (to:nat{ from <= to /\ to <= k })
+: Tot (s:idx_set m n { forall (j:nat { from <= j /\ j < to }). select p j `Set.subset` s })
+      (decreases to - from)
+= if from = to then Set.emptyset
+  else Set.union (p from) (union_partitions_aux p (from + 1 <: nat) to)
+let union_partitions #m #n #k (p:partitions m n k) = union_partitions_aux p 0 k
 
-let disjoint_partitions (m:nat) (n:nat) =
-  l:seq (idx_set m n) {
-    m <= n  /\
-    (forall (i j:nat). {:pattern (Seq.index l i); (Seq.index l j)}
-       i < j /\ j < Seq.length l ==> OrdSet.disjoint (Seq.index l i) (Seq.index l j)) /\
-    (union_partitions l `OrdSet.equal` range m n)
+let rec range (m:nat) (n:nat { m <= n }) 
+: Tot (s:idx_set m n { forall x. Set.mem x s <==> m <= x /\ x < n }) (decreases n - m)
+= if m = n then Set.emptyset
+  else Set.union (Set.singleton m) (range (m + 1) n)
+
+let parts_disjoint #m #n #k (parts:partitions m n k) =
+  forall (i j:nat). {:pattern (select parts i); (select parts j) }
+      i < j /\ j < k ==> Set.disjoint (select parts i) (select parts j)
+
+let parts_covers_range_except #m #n #k (parts:partitions m n k) (except:Set.set nat) =
+  m <= n /\
+  Set.difference (range m n) except `Set.subset` union_partitions parts
+
+let parts_covers_range #m #n #k (parts:partitions m n k) =
+  parts_covers_range_except parts Set.emptyset
+
+let disjoint_partitions (m:nat) (n:nat) (k:nat) =
+  parts:partitions m n k {
+    parts_disjoint parts /\
+    parts_covers_range parts
   }
 
-let star_over_partition (m:nat) (n:nat{m<n}) (f:idx m n -> slprop) (partition:idx_set m n)
-: slprop
-= f m
+let rec star_over_partition (#m:nat) (#n:nat{m<=n}) (f:idx m n -> slprop) (partition:idx_set m n)
+: Tot slprop (decreases (cardinality partition))
+= if cardinality partition = 0
+  then emp
+  else (
+    let i = Set.choose partition in
+    let partition' = Set.remove i partition in
+    f i ** star_over_partition f partition'
+  )
 
- 
-// ghost
-// fn bigstar_rewrite
-//   (m0:nat)
-//   (n0:nat{m0 <= n0})
-//   (m1:nat)
-//   (n1:nat{m1 <= n1})
-//   (f0: (i:nat { m0 <= i /\ i < n0 } -> slprop))
-//   (f1: (i:nat { m1 <= i /\ i < n1 } -> slprop))
-//   (partition: disjoint_partitions m0 n0)
-// requires
-//   bigstar m0 n0 f0
-//   pure (forall (i:nat { m1 <= i /\ i < n1 }). f1 i == f0 i)
-// ensures
-//   bigstar m1 n1 f1
-// {
-//   admit()
-// }
+let partition_range (n:nat { n % 2 == 0 })
+: partitions 0 n (n / 2)
+= fun i -> Set.union (Set.singleton i) (Set.singleton (n - i - 1))
+
+let star_over_partition_range (n:nat { n % 2 == 0 }) (f:idx 0 n -> slprop) (i:nat { i < n / 2 })
+: Lemma
+  (ensures star_over_partition f (select (partition_range n) i) ==
+            f i ** f (n - i - 1 <: nat))
+= slprop_equivs() 
+
+let partition_range_disjoint (n:nat { n % 2 == 0 })
+: Lemma (parts_disjoint (partition_range n))
+= ()
+
+#restart-solver
+#push-options "--query_stats --fuel 0 --ifuel 0"
+let partition_covers_range_lemma (n:nat { n % 2 == 0 })
+: Lemma (ensures parts_covers_range (partition_range n))
+= introduce forall z. z `Set.mem` range 0 n ==> z `Set.mem` union_partitions (partition_range n)
+  with introduce _ ==> _
+  with _. (
+    if z < n / 2
+    then (
+      assert (z `Set.mem` select (partition_range n) z)
+    )
+    else (
+      assert (z `Set.mem` select (partition_range n) (n - z - 1 <: nat))
+    )
+  )
+#pop-options
+
+let disjoint_partitions_range (n:nat { n % 2 == 0 })
+: disjoint_partitions 0 n (n / 2)
+= partition_range_disjoint n;
+  partition_covers_range_lemma n;
+  partition_range n
+
+ghost
+fn bigstar_partition
+  (n0:nat)
+  (n1:nat)
+  (f0: (idx 0 n0 -> slprop))
+  (partition: disjoint_partitions 0 n0 n1)
+requires
+  bigstar 0 n0 f0
+ensures
+  bigstar 0 n1 (fun i -> star_over_partition f0 (select partition i))
+{
+  admit()
+}
+
+ghost
+fn bigstar_partition_inv
+  (n0:nat)
+  (n1:nat)
+  (f0: (idx 0 n0 -> slprop))
+  (partition: disjoint_partitions 0 n0 n1)
+requires
+ bigstar 0 n1 (fun i -> star_over_partition f0 (select partition i))
+ensures
+  bigstar 0 n0 f0
+{
+  admit()
+}
 
 let gpu_pts_to_cell
   (#a:Type0)
   (#sz:nat)
   (arr : gpu_array a sz)
-  (#[exact (`1.0R)] f : perm)
+  (#f : perm)
   (i:nat)
   (v:a)
 : slprop
@@ -100,52 +163,182 @@ ensures
     slice_to_cell;
 }
 
-fn read_cell_named
+
+ghost
+fn implode_cells
+  (#a:Type0)
+  (#sz:nat)
+  (arr : gpu_array a sz)
+  (#f : perm)
+  (#s:seq a { Seq.length s == sz })
+requires
+  bigstar 0 sz (fun (i:idx 0 sz) -> gpu_pts_to_cell arr #f i (Seq.index s i))
+ensures
+  gpu_pts_to_array arr #f s
+{
+  ghost
+  fn cell_to_slice (i:nat { 0 <= i /\ i < sz })
+  requires
+    gpu_pts_to_cell arr #f i (Seq.index s i)
+  ensures
+    gpu_pts_to_array_slice arr #f i (Prims.op_Addition i 1) seq![Seq.index s i]
+  {
+    unfold (gpu_pts_to_cell arr #f i (Seq.index s i));
+    with s'. assert (gpu_pts_to_array_slice arr #f i (i+1) s');
+    assert pure (reveal s' `Seq.equal` seq![Seq.index (reveal s) i]);
+  };
+  bigstar_map
+    #_ #_ #0 #sz
+    #(fun (i:idx 0 sz) -> gpu_pts_to_cell arr #f i (Seq.index s i))
+    #(fun i -> gpu_pts_to_array_slice arr #f i (Prims.op_Addition i 1) seq![Seq.index s i])
+    cell_to_slice;
+  gpu_array_unslice_1 arr #f #s
+}
+
+
+#push-options "--print_implicits --print_bound_var_types"
+
+ghost
+fn partition_cells
+  (#a:Type0)
+  (#size:sz { size % 2sz == 0sz })
+  (arr : gpu_array a size)
+  (#f : perm)
+  (#s:seq a { Seq.length s == SZ.v size })
+requires
+  bigstar 0 size (fun i ->
+    gpu_pts_to_cell arr #f i (Seq.index s i))
+ensures
+  bigstar 0 (SZ.v (size `div` 2sz)) (fun i ->
+    gpu_pts_to_cell arr #f i (Seq.index s i) **
+    gpu_pts_to_cell arr #f (SZ.v size - i - 1) (index_flip s i))
+{ 
+  bigstar_partition size (size `div` 2sz)
+    (fun i -> gpu_pts_to_cell arr #f i (Seq.index s i))
+    (disjoint_partitions_range size);
+  
+  ghost
+  fn star_over_partition_range
+      (n:nat { n % 2 == 0 })
+      (f:idx 0 n -> slprop)
+      (i:nat { 0 <= i /\ i < n / 2 })
+  requires 
+    star_over_partition f (select (disjoint_partitions_range n) i)
+  ensures
+    f i ** f (n - i - 1 <: nat)
+  {
+    star_over_partition_range n f i;
+    rewrite 
+       (star_over_partition f (select (disjoint_partitions_range n) i))
+    as (f i ** f (n - i - 1 <: nat))
+  };
+
+  bigstar_map
+    #0 #_ #0 #(size `div` 2sz)
+    #(fun i -> 
+      star_over_partition
+        (fun i -> gpu_pts_to_cell arr #f i (Seq.index s i))
+        (select (disjoint_partitions_range size) i))
+    #(fun i ->
+      gpu_pts_to_cell arr #f i (Seq.index s i) **
+      gpu_pts_to_cell arr #f (SZ.v size - i - 1) (index_flip s i))
+    (star_over_partition_range
+        size
+        (fun i -> gpu_pts_to_cell arr #f i (Seq.index s i)));
+}
+
+ghost
+fn partition_cells_inv
+ (#a:Type0)
+  (#size:sz { size % 2sz == 0sz })
+  (arr : gpu_array a size)
+  (#f : perm)
+  (#s:seq a { Seq.length s == SZ.v size })
+requires
+  bigstar 0 (SZ.v (size `div` 2sz)) (fun i ->
+    gpu_pts_to_cell arr #f i (Seq.index s i) **
+    gpu_pts_to_cell arr #f (SZ.v size - i - 1) (index_flip s i))
+ensures
+  bigstar 0 size (fun (i:idx 0 (SZ.v size)) ->
+    gpu_pts_to_cell arr #f i (Seq.index s i))
+{ 
+  ghost
+  fn star_over_partition_range_inv
+      (n:nat { n % 2 == 0 })
+      (f:idx 0 n -> slprop)
+      (i:nat { 0 <= i /\ i < n / 2 })
+  requires 
+    f i ** f (n - i - 1 <: nat)
+  ensures
+    star_over_partition f (select (partition_range n) i)
+  {
+    star_over_partition_range n f i;
+    rewrite 
+        (f i ** f (n - i - 1 <: nat))
+     as (star_over_partition f (select (partition_range n) i))
+  };
+ 
+  bigstar_map
+    #_ #_ #0 #(size `div` 2sz)
+    #(fun i -> 
+      gpu_pts_to_cell arr #f i (Seq.index s i) **
+      gpu_pts_to_cell arr #f (SZ.v size - i - 1) (index_flip s i))
+    #(fun i -> 
+      star_over_partition
+        (fun i -> gpu_pts_to_cell arr #f i (Seq.index s i))
+        (select (partition_range size) i))
+    (star_over_partition_range_inv
+        size
+        (fun i -> gpu_pts_to_cell arr #f i (Seq.index s i)));
+
+  bigstar_partition_inv size (size `div` 2sz)
+      (fun i -> gpu_pts_to_cell arr #f i (Seq.index s i))
+      (disjoint_partitions_range size);
+
+
+}
+
+fn read_cell
   (#ty:Type0)
   (#size:erased sz)
   (a:gpu_array ty (SZ.v size))
   (i:sz { i < size })
-  (#name:string)
+  (#p:perm)
   (#u:erased ty)
 requires
   gpu **
-  named name (gpu_pts_to_cell a (SZ.v i) u)
+  gpu_pts_to_cell a #p (SZ.v i) u
 returns v:ty
 ensures
   gpu **
-  named name (gpu_pts_to_cell a (SZ.v i) u) **
+  gpu_pts_to_cell a #p (SZ.v i) u **
   pure (u == v)
 {
-  unfold named;
-  unfold (gpu_pts_to_cell a (SZ.v i) u);
+  unfold gpu_pts_to_cell; //a (SZ.v i) u);
   //Why do I have to instantiate the implicits?
   let v = gpu_array_read #_ #_ #(SZ.v i) #(SZ.v i + 1) a i;
-  fold (gpu_pts_to_cell a (SZ.v i) u);
-  fold (named name (gpu_pts_to_cell a (SZ.v i) u));
+  fold (gpu_pts_to_cell a #p (SZ.v i) u);
   v
 }
 
-fn write_cell_named
+fn write_cell
   (#ty:Type0)
   (#size:erased sz)
   (a:gpu_array ty (SZ.v size))
   (i:sz { i < size })
   (v:ty)
-  (#name:string)
   (#u:erased ty)
 requires
   gpu **
-  named name (gpu_pts_to_cell a (SZ.v i) u)
+  gpu_pts_to_cell a #1.0R (SZ.v i) u
 ensures
   gpu **
-  named name (gpu_pts_to_cell a (SZ.v i) v)
+  gpu_pts_to_cell a #1.0R (SZ.v i) v
 {
-  unfold named;
-  unfold (gpu_pts_to_cell a (SZ.v i) u);
+  unfold gpu_pts_to_cell;
   //Why do I have to instantiate the implicits?
   gpu_array_write #_ #_ #(SZ.v i) #(SZ.v i + 1) a i v;
-  fold (gpu_pts_to_cell a (SZ.v i) v);
-  fold (named name (gpu_pts_to_cell a (SZ.v i) v))
+  fold (gpu_pts_to_cell a #1.0R (SZ.v i) v);
 }
 
 
@@ -154,31 +347,30 @@ fn kernel
   (#ty:Type0)
   (size:sz)
   (a:gpu_array ty size)
-  (etid:erased tid_t { bidx_x etid < size `div` 2sz /\ gdim_x etid == 1sz })
-  (#u #v:erased ty)
+  (#s:erased (Seq.seq ty) { Seq.length s == SZ.v size })
+  (etid:tid_t { gdim_x etid == size `div` 2sz /\ bdim_x etid == 1sz }) //thread_index etid < SZ.v size / 2 })
 requires
   gpu **
   thread_id etid **
-  named "cell_l" (gpu_pts_to_cell a (bidx_x etid) u) **
-  named "cell_r" (gpu_pts_to_cell a (size - bidx_x etid - 1sz) v)
+  (gpu_pts_to_cell a #1.0R (thread_index etid) (Seq.index s (thread_index etid)) **
+   gpu_pts_to_cell a #1.0R (SZ.v size - thread_index etid - 1) (index_flip s (thread_index etid)))
 ensures
   gpu **
   thread_id etid **
-  named "cell_l" (gpu_pts_to_cell a (bidx_x etid) v) **
-  named "cell_r" (gpu_pts_to_cell a (size - bidx_x etid - 1sz) u)
+  (gpu_pts_to_cell a #1.0R (thread_index etid) (Seq.index (reverse_spec s) (thread_index etid)) **
+   gpu_pts_to_cell a #1.0R (SZ.v size - thread_index etid - 1sz) (index_flip (reverse_spec s) (thread_index etid)))
 {
-  let tid = GPU.Base.block_idx_x ();
-  let idx = uint32_to_sizet tid;
+  let idx = GPU.Base.thread_idx_all ();
   let idx' = (size - idx - 1sz);
-  let uu = read_cell_named a idx #"cell_l";
-  let vv = read_cell_named a idx' #"cell_r";
-  write_cell_named a idx vv #"cell_l";
-  write_cell_named a idx' uu #"cell_r"
+  let uu = read_cell a idx;
+  let vv = read_cell a idx';
+  write_cell a idx vv;
+  write_cell a idx' uu;
 }
 
 fn reverse
     (#ty:Type0)
-    (size:sz { size % 2sz == 0sz /\ SZ.v size < max_blocks })
+    (size:sz { size > 0sz /\ size % 2sz == 0sz /\ SZ.v size < max_blocks })
     (a:gpu_array ty size)
     (#s:FStar.Seq.seq ty { Seq.length s == SZ.v size })
 requires
@@ -186,9 +378,19 @@ requires
   gpu_pts_to_array a s
 ensures
   cpu **
-  gpu_pts_to_array a s
+  gpu_pts_to_array a (reverse_spec s)
 {
   explode_cells a;
-  admit();
-  ()
+  partition_cells a;
+  launch_kernel_n
+    (size `div` 2sz) 
+    #(fun tid -> 
+      gpu_pts_to_cell a #1.0R tid (Seq.index s tid) **
+      gpu_pts_to_cell a #1.0R (SZ.v size - tid - 1) (index_flip s tid))
+    #(fun tid -> 
+      gpu_pts_to_cell a #1.0R tid (Seq.index (reverse_spec s) tid) **
+      gpu_pts_to_cell a #1.0R (SZ.v size - tid - 1) (index_flip (reverse_spec s) tid))
+    (kernel size a #s);
+  partition_cells_inv a;
+  implode_cells a
 }
